Julek/mtl point mul and add into dest (#36)

src/specs/PointMulAndAddIntoDest.ec
@@ -35,6 +35,23 @@ module PointMulAndAddIntoDest = {
       RevertWithMessage.low(W256.of_int 22, W256.of_int STRING);
     }
   }
+
+  proc mid(x1 : int, y1 : int, s : int, x2 : int, y2 : int) : (int * int) option = {
+      var x1_F, y1_F, x2_F, y2_F, mresult, mresult', aresult, fresult; 
+      x1_F <- ZModField.inzmod x1;
+      y1_F <- ZModField.inzmod y1;
+      mresult <- ecMul_precompile x1_F y1_F s;
+      if (is_some mresult) {
+         x2_F <- ZModField.inzmod x2;
+         y2_F <- ZModField.inzmod y2;
+         mresult' <- odflt (ZModField.zero, ZModField.zero) mresult;
+         aresult  <- ecAdd_precompile mresult'.`1 mresult'.`2 x2_F y2_F; 
+         fresult <- omap F_to_int_point aresult;
+      } else {
+          fresult <- None;
+      }
+      return fresult;
+  }
 }.
 
 lemma pointMulAndAddIntoDest_extracted_equiv_low :
@@ -53,3 +70,572 @@ proof.
   inline*. wp. skip. by progress.
   inline*. wp. skip. by progress.
 qed.
+  
+lemma PointMulAndAddIntoDest_mid_of_low (x1v y1v x2v y2v sv : int) (p1u destu : uint256) (memory0 : MemoryMap.mem) : equiv [
+    PointMulAndAddIntoDest.low ~ PointMulAndAddIntoDest.mid :
+    Primops.memory{1} = memory0 /\
+      0 <= x1v < p /\ 0 <= y1v < p /\ 0 <= sv < W256.modulus /\ 0 <= x2v < p /\ 0 <= y2v < p /\
+      (of_int 128)%W256 <= p1u /\
+      (of_int 64)%W256 <= -p1u /\
+      (of_int 128)%W256 <= p1u + (of_int 32)%W256 /\
+      (of_int 32)%W256 <= - (p1u + (of_int 32)%W256) /\
+      (of_int 128)%W256 <= destu /\
+      (of_int 64)%W256 <= -destu /\
+      (of_int 128)%W256 <= destu + (of_int 32)%W256 /\
+      (of_int 32)%W256 <= - (destu + (of_int 32)%W256) /\
+    PurePrimops.mload memory0 p1u = W256.of_int x1v /\
+    PurePrimops.mload memory0 (p1u + W256.of_int 32) = W256.of_int y1v /\
+    PurePrimops.mload memory0 destu = W256.of_int x2v /\
+    PurePrimops.mload memory0 (destu + W256.of_int 32) = W256.of_int y2v /\
+      arg{1} = (p1u, W256.of_int sv, destu) /\ arg{2} = (x1v, y1v, sv, x2v, y2v) /\ !Primops.reverted{1}
+      ==>
+      (
+        ConcretePrimops.staticcall_ec_mul_should_succeed (W256.of_int x1v, W256.of_int y1v) (W256.of_int sv) /\
+        exists (x y : F),
+        ecMul_precompile (ZModField.inzmod x1v) (ZModField.inzmod y1v) sv = Some (x, y) /\
+        (
+          ConcretePrimops.staticcall_ec_add_should_succeed (W256.of_int (ZModField.asint x), W256.of_int (ZModField.asint y)) (W256.of_int x2v, W256.of_int y2v) /\
+          exists (x' y' : F),
+          ecAdd_precompile x y (ZModField.inzmod x2v) (ZModField.inzmod y2v) = Some (x', y') /\
+          res{2} = Some( F_to_int_point (x', y')) /\
+          Primops.memory{1} = PurePrimops.mstore (PurePrimops.mstore (PurePrimops.mstore (PurePrimops.mstore (PurePrimops.mstore (PurePrimops.mstore memory0 W256.zero (W256.of_int (ZModField.asint x))) (W256.of_int 32) (W256.of_int (ZModField.asint y))) (W256.of_int 64) (W256.of_int x2v)) (W256.of_int 96) (W256.of_int y2v)) destu (W256.of_int (ZModField.asint x'))) (destu + W256.of_int 32) (W256.of_int (ZModField.asint y')) /\ 
+          !Primops.reverted{1}
+        )
+        \/
+        (
+          !ConcretePrimops.staticcall_ec_add_should_succeed (W256.of_int (ZModField.asint x), W256.of_int (ZModField.asint y)) (W256.of_int x2v, W256.of_int y2v) /\
+          res{2} = None /\
+          Primops.reverted{1}
+        )
+      ) \/
+      (
+        !ConcretePrimops.staticcall_ec_mul_should_succeed (W256.of_int x1v, W256.of_int y1v) (W256.of_int sv) /\
+        res{2} = None /\
+        Primops.reverted{1}
+      )
+    ]. proof.
+    proc.
+        seq 6 2 :
+    (
+      0 <= x1v < p /\ 0 <= y1v < p /\ 0 <= sv < W256.modulus /\ 0 <= x2v < p /\ 0 <= y2v < p /\
+      (of_int 128)%W256 <= destu /\
+      (of_int 64)%W256 <= -destu /\
+      (of_int 128)%W256 <= destu + (of_int 32)%W256 /\
+      (of_int 32)%W256 <= - (destu + (of_int 32)%W256) /\
+      PurePrimops.mload memory0 destu = W256.of_int x2v /\
+      PurePrimops.mload memory0 (destu + W256.of_int 32) = W256.of_int y2v /\
+      Primops.memory{1} = PurePrimops.mstore (PurePrimops.mstore (PurePrimops.mstore memory0 W256.zero (W256.of_int x1v)) (W256.of_int 32) (W256.of_int y1v)) (W256.of_int 64) (W256.of_int sv) /\
+      x1_F{2} = ZModField.inzmod x1v /\ y1_F{2} = ZModField.inzmod y1v /\
+      (point{1}, s{1}, dest{1}) = (p1u, W256.of_int sv, destu) /\ (x1{2}, y1{2}, s{2}, x2{2}, y2{2}) = (x1v, y1v, sv, x2v, y2v) /\ !Primops.reverted{1}
+    ).
+        inline *. wp. skip. progress. congr.
+
+        rewrite MemoryMap.load_store_diff. smt (@W256 @Utils). smt (@W256 @Utils).
+        rewrite H17 H18. reflexivity.
+
+        case (ConcretePrimops.staticcall_ec_mul_should_succeed (W256.of_int x1v, W256.of_int y1v) (W256.of_int sv)).
+
+        seq 1 1 :
+    (
+      (0 <= x1v && x1v < p) /\
+      (0 <= y1v && y1v < p) /\
+      (0 <= sv && sv < W256.modulus) /\
+      (0 <= x2v && x2v < p) /\
+      (0 <= y2v && y2v < p) /\
+        W256.of_int 128 <= destu /\
+        W256.of_int 64  <= -destu /\
+        W256.of_int 128 <= destu + (W256.of_int 32) /\
+        W256.of_int 32  <= - (destu + (W256.of_int 32)) /\
+        PurePrimops.mload memory0 destu = W256.of_int x2v /\
+        PurePrimops.mload memory0 (destu + (W256.of_int 32)) = W256.of_int y2v /\
+      x1_F{2} = ZModField.inzmod x1v /\
+      y1_F{2} = ZModField.inzmod y1v /\
+        (point{1}, s{1}, dest{1}) = (p1u, W256.of_int sv, destu) /\
+        (x1{2}, y1{2}, s{2}, x2{2}, y2{2}) = (x1v, y1v, sv, x2v, y2v) /\
+          !Primops.reverted{1} /\
+        (ConcretePrimops.staticcall_ec_mul_should_succeed (W256.of_int x1v, W256.of_int y1v)
+          (W256.of_int sv)) /\
+            exists (x y : F),
+        ecMul_precompile x1_F{2} y1_F{2} sv = Some (x, y) /\
+        success{1} = W256.one /\ mresult{2} = Some (x, y) /\
+            Primops.memory{1} =
+        (PurePrimops.mstore
+          ((PurePrimops.mstore ((PurePrimops.mstore memory0 W256.zero ((W256.of_int (ZModField.asint x)))))
+              (W256.of_int 32) (W256.of_int (ZModField.asint y))))
+          (W256.of_int 64) (W256.of_int sv))
+      ).
+
+          exists* Primops.memory{1}.
+          elim*=> memory1.
+          seq 0 0 :
+      (
+        exists (x y : F),
+        ecMul_precompile (ZModField.inzmod x1v) (ZModField.inzmod y1v) sv = Some (x, y) /\
+        memory1 = Primops.memory{1} /\
+        ((0 <= x1v && x1v < p) /\
+          (0 <= y1v && y1v < p) /\
+          (0 <= sv && sv < W256.modulus) /\
+          (0 <= x2v && x2v < p) /\
+          (0 <= y2v && y2v < p) /\
+          (of_int 128)%W256 <= destu /\
+          (of_int 64)%W256 <= -destu /\
+          (of_int 128)%W256 <= destu + (W256.of_int 32) /\
+          (of_int 32)%W256 <= - (destu + (W256.of_int 32)) /\
+          PurePrimops.mload memory0 destu = W256.of_int x2v /\
+          PurePrimops.mload memory0 (destu + (W256.of_int 32)) = (W256.of_int y2v) /\
+            Primops.memory{1} =
+          (PurePrimops.mstore
+            ((PurePrimops.mstore ((PurePrimops.mstore memory0 W256.zero ((of_int x1v))%W256))
+                ((of_int 32))%W256 ((of_int y1v))%W256))%PurePrimops
+            ((of_int 64))%W256 ((of_int sv))%W256)%PurePrimops /\
+          x1_F{2} = (ZModField.inzmod x1v) /\
+          y1_F{2} = (ZModField.inzmod y1v) /\
+          (point{1}, s{1}, dest{1}) = (p1u, (of_int sv)%W256, destu) /\
+          (x1{2}, y1{2}, s{2}, x2{2}, y2{2}) = (x1v, y1v, sv, x2v, y2v) /\
+            !Primops.reverted{1}) /\
+        (ConcretePrimops.staticcall_ec_mul_should_succeed ((of_int x1v)%W256, (of_int y1v)%W256)
+          ((of_int sv))%W256)
+      ). skip. progress. 
+          have J0 := exists_of_is_some _ (ConcretePrimops.ecMul_precomp_is_some_of_should_succeed _ _ H16).
+          case J0. move=>pt J0. pose x := pt.`1. pose y := pt.`2. exists x. exists y.
+          progress.
+          have J0' : ecMul_precompile
+      (ZModField.inzmod (to_uint (W256.of_int x1{2})))
+      (ZModField.inzmod (to_uint (W256.of_int y1{2})))
+      (to_uint (W256.of_int s{2})) =
+        Some pt. smt ().
+        rewrite to_uint_small in J0'. progress. apply (lt_trans _ p _). exact H0. exact p_lt_W256_mod.
+        rewrite to_uint_small in J0'. progress. apply (lt_trans _ p _). exact H2. exact p_lt_W256_mod.
+        rewrite to_uint_small in J0'. progress. smt ().
+        elim* => x y.
+      
+        call {1} (ConcretePrimops.staticcall_ec_mul_pspec memory1 (W256.of_int x1v, W256.of_int y1v) (W256.of_int sv) W256.zero W256.zero). wp. skip. progress. 
+
+          rewrite MemoryMap.load_store_diff. smt (@W256 @Utils). smt (@W256 @Utils).
+          rewrite MemoryMap.load_store_diff. smt (@W256 @Utils). smt (@W256 @Utils).
+          rewrite MemoryMap.load_store_same. reflexivity.
+
+          rewrite MemoryMap.load_store_diff. smt (@W256 @Utils). smt (@W256 @Utils).
+          rewrite MemoryMap.load_store_same. reflexivity.
+
+          rewrite MemoryMap.load_store_same. reflexivity.
+
+        exists x. exists y. progress. smt ().
+        have J1 :
+      (
+        memory_L =
+     (PurePrimops.mstore
+        ((PurePrimops.mstore
+            ((PurePrimops.mstore
+                ((PurePrimops.mstore
+                    ((PurePrimops.mstore memory0 W256.zero ((of_int x1{2}))%W256))
+                    ((of_int 32))%W256 ((of_int y1{2}))%W256))%PurePrimops
+                ((of_int 64))%W256 ((of_int s{2}))%W256))%PurePrimops
+            W256.zero
+            ((ConcretePrimops.ecMul_precompile_unsafe_cast
+                ((of_int x1{2})%W256, (of_int y1{2})%W256)
+                ((of_int s{2}))%W256)).`1))%PurePrimops
+        ((of_int 32))%W256
+        ((ConcretePrimops.ecMul_precompile_unsafe_cast
+            ((of_int x1{2})%W256, (of_int y1{2})%W256) ((of_int s{2}))%W256)).`2)%PurePrimops
+    ). smt ().
+
+        rewrite J1.
+        rewrite -(MemoryMap.store_store_swap_diff _ W256.zero). smt (@W256 @Utils). smt (@W256 @Utils).
+        rewrite -(MemoryMap.store_store_swap_diff _ W256.zero). smt (@W256 @Utils). smt (@W256 @Utils).
+        rewrite MemoryMap.store_store_same.
+
+        rewrite -(MemoryMap.store_store_swap_diff _ (W256.of_int 32)). smt (@W256 @Utils). smt (@W256 @Utils).
+        rewrite MemoryMap.store_store_same. 
+        rewrite /ecMul_precompile_unsafe_cast. simplify.
+        rewrite to_uint_small. progress. apply (lt_trans _ p _). exact H1. exact p_lt_W256_mod.
+        rewrite to_uint_small. progress. apply (lt_trans _ p _). exact H3. exact p_lt_W256_mod.
+        rewrite to_uint_small. progress.
+
+        rewrite H. progress.
+
+        rcondt {2} 1. progress.
+
+        seq 5 3 :
+    (
+      exists (x y : F),
+      (0 <= x1v && x1v < p) /\
+      (0 <= y1v && y1v < p) /\
+      (0 <= sv && sv < W256.modulus) /\
+      (0 <= x2v && x2v < p) /\
+      (0 <= y2v && y2v < p) /\
+      x2_F{2} = ZModField.inzmod x2v /\
+      y2_F{2} = ZModField.inzmod y2v /\
+      (point{1}, s{1}, dest{1}) = (p1u, W256.of_int sv, destu) /\
+      (x1{2}, y1{2}, s{2}, x2{2}, y2{2}) = (x1v, y1v, sv, x2v, y2v) /\
+        !Primops.reverted{1} /\
+      (ConcretePrimops.staticcall_ec_mul_should_succeed (W256.of_int x1v, W256.of_int y1v)
+        (W256.of_int sv)) /\
+          ecMul_precompile (ZModField.inzmod x1v) (ZModField.inzmod y1v) sv = Some (x, y) /\
+      success{1} = W256.one /\
+      mresult'{2} = (x, y) /\
+          Primops.memory{1} =
+          PurePrimops.mstore (PurePrimops.mstore
+        (PurePrimops.mstore
+          (PurePrimops.mstore memory0 W256.zero (W256.of_int (ZModField.asint x)))
+          (W256.of_int 32) (W256.of_int (ZModField.asint y)))
+        (W256.of_int 64) (W256.of_int x2v)) (W256.of_int 96) (W256.of_int y2v)
+    ).
+
+          inline *. wp. skip. progress.
+          exists x. exists y.
+          progress.
+
+      
+        rewrite MemoryMap.load_store_diff.
+    
+        rewrite Utils.uint_256_cast_sub.
+        apply uint256_le_of_le.
+        rewrite to_uint_small. smt ().
+        rewrite to_uint_small. smt (@IntDiv @W256).
+        rewrite to_uint_small. smt ().
+        have H9' : 128 <= to_uint dest{1}. smt (@W256 @Utils).
+        have J0 : to_uint dest{1} < W256.modulus. apply uint256_size.
+        rewrite mod_eq_self. smt (). smt (). apply sub_mono_lt. smt (). exact J0. smt ().
+
+        rewrite Utils.uint_256_cast_sub.
+        apply uint256_le_of_le.
+        rewrite to_uint_small. smt ().
+        rewrite to_uint_small. smt ().
+        rewrite to_uint_small. smt ().
+        have H9' : 128 <= to_uint dest{1}. smt (@W256 @Utils).
+        have J0 : to_uint dest{1} < W256.modulus. apply uint256_size.
+        rewrite mod_plus.
+        rewrite mod_eq_self. smt (). smt. smt. smt.
+
+        rewrite MemoryMap.load_store_diff.
+
+        rewrite Utils.uint_256_cast_sub.
+        apply uint256_le_of_le.
+        rewrite to_uint_small. smt ().
+        rewrite to_uint_small. smt (@IntDiv @W256).
+        have H9' : 128 <= to_uint dest{1}. smt (@W256 @Utils).
+        have J0 : to_uint dest{1} < W256.modulus. apply uint256_size.
+        rewrite mod_eq_self. smt (). smt (). smt. smt ().
+
+        rewrite Utils.uint_256_cast_sub.
+        apply uint256_le_of_le.
+        rewrite to_uint_small. smt ().
+        rewrite to_uint_small. smt ().
+        have H9' : 128 <= to_uint dest{1}. smt (@W256 @Utils).
+        have J0 : to_uint dest{1} < W256.modulus. apply uint256_size.
+        rewrite mod_plus.
+        rewrite mod_eq_self. smt (). smt. smt. smt.
+
+        rewrite MemoryMap.load_store_diff.
+
+        smt (@W256 @Utils).
+        smt (@W256 @Utils).
+
+        rewrite MemoryMap.load_store_diff.
+
+        have J0 : dest{1} + (of_int 32)%W256 - (of_int 64)%W256 = dest{1} - (of_int 32)%W256. smt (@Utils @W256).
+        rewrite J0.
+        rewrite Utils.uint_256_cast_sub.
+        apply uint256_le_of_le.
+        rewrite to_uint_small. smt ().
+        rewrite to_uint_small. smt (@IntDiv @W256).
+        have H9' : 128 <= to_uint dest{1}. smt (@W256 @Utils).
+        have J1 : to_uint dest{1} < W256.modulus. apply uint256_size.
+        rewrite mod_eq_self. smt (). smt (). smt. smt ().
+
+        have K0 : (of_int 64)%W256 - (dest{1} + (of_int 32)%W256) = (W256.of_int 32) - dest{1}.
+        rewrite uint256_distrib_sub. smt (@W256 @Utils).
+        rewrite K0.
+        rewrite Utils.uint_256_cast_sub.
+        apply uint256_le_of_le.
+        rewrite to_uint_small. smt ().
+        rewrite to_uint_small. smt ().
+        have H9' : 128 <= to_uint dest{1}. smt (@W256 @Utils).
+        have J0 : to_uint dest{1} < W256.modulus. apply uint256_size.
+        rewrite mod_plus.
+        rewrite mod_eq_self. smt (). smt. smt. smt.
+
+        rewrite MemoryMap.load_store_diff.
+    
+        have J0 : dest{1} + (of_int 32)%W256 - (of_int 64)%W256 = dest{1} - (of_int 32)%W256. smt (@Utils @W256).
+        rewrite J0.
+        rewrite Utils.uint_256_cast_sub.
+        apply uint256_le_of_le.
+        rewrite to_uint_small. smt ().
+        rewrite to_uint_small. smt (@IntDiv @W256).
+        have H9' : 128 <= to_uint dest{1}. smt (@W256 @Utils).
+        have J1 : to_uint dest{1} < W256.modulus. apply uint256_size.
+        rewrite mod_eq_self. smt (). smt (). smt. smt ().
+
+        have K0 : (of_int 64)%W256 - (dest{1} + (of_int 32)%W256) = (W256.of_int 32) - dest{1}.
+        rewrite uint256_distrib_sub. smt (@W256 @Utils).
+        rewrite K0.
+        rewrite Utils.uint_256_cast_sub.
+        apply uint256_le_of_le.
+        rewrite to_uint_small. smt ().
+        rewrite to_uint_small. smt ().
+        have H9' : 128 <= to_uint dest{1}. smt (@W256 @Utils).
+        have J0 : to_uint dest{1} < W256.modulus. apply uint256_size.
+        rewrite mod_plus.
+        rewrite mod_eq_self. smt (). smt. smt. smt.
+
+        rewrite MemoryMap.load_store_diff.
+        smt (@W256 @Utils).
+        smt (@W256 @Utils).
+
+        rewrite MemoryMap.load_store_diff.
+        smt (@W256 @Utils).
+        smt (@W256 @Utils).
+    
+    
+        smt (@MemoryMap).
+        elim*=> x y.
+
+        case (ConcretePrimops.staticcall_ec_add_should_succeed (W256.of_int (ZModField.asint x), W256.of_int (ZModField.asint y)) (W256.of_int x2v, W256.of_int y2v)).
+
+        seq 0 0 :
+    (
+      exists (x' y' : F),
+      ((0 <= x1v && x1v < p) /\
+        (0 <= y1v && y1v < p) /\
+        (0 <= sv && sv < W256.modulus) /\
+        (0 <= x2v && x2v < p) /\
+        (0 <= y2v && y2v < p) /\
+        x2_F{2} = ZModField.inzmod x2v /\
+        y2_F{2} = ZModField.inzmod y2v /\
+        (point{1}, s{1}, dest{1}) = (p1u, (of_int sv)%W256, destu) /\
+        (x1{2}, y1{2}, s{2}, x2{2}, y2{2}) = (x1v, y1v, sv, x2v, y2v) /\
+          !Primops.reverted{1} /\
+        (ConcretePrimops.staticcall_ec_mul_should_succeed (W256.of_int x1v, W256.of_int y1v)
+          (W256.of_int sv)) /\
+            ecMul_precompile (ZModField.inzmod x1v) (ZModField.inzmod y1v) sv =
+            Some (x, y) /\
+            ecAdd_precompile x y (ZModField.inzmod x2v) (ZModField.inzmod y2v) =
+            Some (x', y') /\
+        success{1} = W256.one /\
+        mresult'{2} = (x, y) /\
+            Primops.memory{1} =
+        (PurePrimops.mstore
+          ((PurePrimops.mstore
+              ((PurePrimops.mstore
+                  ((PurePrimops.mstore memory0 W256.zero
+                      (W256.of_int (ZModField.asint x))))
+                  ((of_int 32))%W256 ((of_int ((ZModField.asint y))))%W256))%PurePrimops
+              ((of_int 64))%W256 ((of_int x2v))%W256))%PurePrimops
+          ((of_int 96))%W256 ((of_int y2v))%W256)%PurePrimops) /\
+      (ConcretePrimops.staticcall_ec_add_should_succeed
+        ((of_int ((ZModField.asint x)))%W256,
+          (of_int ((ZModField.asint y)))%W256)
+        ((of_int x2v)%W256, (of_int y2v)%W256))
+    ). skip. progress.
+        have H13 := ConcretePrimops.ecAdd_precomp_is_some_of_should_succeed _ _ H12.
+        simplify H13.
+        rewrite proj1 proj1 proj2 proj2 in H13.
+        rewrite to_uint_small in H13. smt.
+        rewrite to_uint_small in H13. smt.
+        rewrite to_uint_small in H13. smt.
+        rewrite to_uint_small in H13. smt.
+        rewrite F_eq_inzmod_asint F_eq_inzmod_asint in H13.
+        have H14 := exists_of_is_some _ H13.
+        case H14. progress.
+        exists v.`1. exists v.`2. progress. smt ().
+
+        elim*=> x' y'.
+    
+          seq 1 1 :
+    (
+        (0 <= x1v && x1v < p) /\
+        (0 <= y1v && y1v < p) /\
+        (0 <= sv && sv < W256.modulus) /\
+        (0 <= x2v && x2v < p) /\
+        (0 <= y2v && y2v < p) /\
+        x2_F{2} = ZModField.inzmod x2v /\
+        y2_F{2} = ZModField.inzmod y2v /\
+        (point{1}, s{1}, dest{1}) = (p1u, (of_int sv)%W256, destu) /\
+        (x1{2}, y1{2}, s{2}, x2{2}, y2{2}) = (x1v, y1v, sv, x2v, y2v) /\
+          !Primops.reverted{1} /\
+        (ConcretePrimops.staticcall_ec_mul_should_succeed ((of_int x1v)%W256, (of_int y1v)%W256)
+          ((of_int sv))%W256) /\
+        success{1} = W256.one /\
+            ecMul_precompile ((ZModField.inzmod x1v)) ((ZModField.inzmod y1v)) sv = Some (x, y) /\
+        mresult'{2} = (x, y) /\
+        ConcretePrimops.staticcall_ec_add_should_succeed (W256.of_int (ZModField.asint x), W256.of_int (ZModField.asint y)) (W256.of_int x2v, W256.of_int y2v) /\
+        _16{1} = W256.one /\
+        ecAdd_precompile x y (ZModField.inzmod x2v) (ZModField.inzmod y2v) = Some (x', y') /\
+        aresult{2} = Some (x', y') /\
+        Primops.memory{1} =
+            PurePrimops.mstore
+            (PurePrimops.mstore 
+            ((PurePrimops.mstore
+              ((PurePrimops.mstore
+                  ((PurePrimops.mstore
+                      ((PurePrimops.mstore memory0 W256.zero
+                          ((of_int ((ZModField.asint x))))%W256))
+                      ((of_int 32))%W256 ((of_int ((ZModField.asint y))))%W256))
+                  ((of_int 64))%W256 ((of_int x2v))%W256))
+              ((of_int 96))%W256 ((of_int y2v))%W256)) destu (W256.of_int (ZModField.asint x'))) (destu + W256.of_int 32) (W256.of_int (ZModField.asint y'))
+    ).
+    
+    
+      
+        exists* Primops.memory{1}.
+        elim*=>memory2. progress.
+      
+        call {1} (ConcretePrimops.staticcall_ec_add_pspec memory2 (W256.of_int (ZModField.asint x), W256.of_int (ZModField.asint y)) (W256.of_int x2v, W256.of_int y2v) W256.zero destu).
+    
+        wp. skip. progress.
+        rewrite MemoryMap.load_store_diff. smt (@W256 @Utils). smt (@W256 @Utils).
+        rewrite MemoryMap.load_store_diff. smt (@W256 @Utils). smt (@W256 @Utils).
+        rewrite MemoryMap.load_store_diff. smt (@W256 @Utils). smt (@W256 @Utils).
+        smt (@MemoryMap).
+
+        rewrite MemoryMap.load_store_diff. smt (@W256 @Utils). smt (@W256 @Utils).
+        rewrite MemoryMap.load_store_diff. smt (@W256 @Utils). smt (@W256 @Utils).
+        smt (@MemoryMap).
+
+        rewrite MemoryMap.load_store_diff. smt (@W256 @Utils). smt (@W256 @Utils).
+        smt (@MemoryMap).
+
+        smt (@MemoryMap).
+
+        smt ().
+
+        have J0 :
+    (
+      memory_L =
+      (PurePrimops.mstore
+        ((PurePrimops.mstore
+            ((PurePrimops.mstore
+                ((PurePrimops.mstore
+                    ((PurePrimops.mstore
+                        ((PurePrimops.mstore memory0 W256.zero
+                            ((W256.of_int (ZModField.asint x)))))
+                        ((W256.of_int 32))
+                        ((W256.of_int ((ZModField.asint y))))))%PurePrimops
+                    ((of_int 64))%W256 ((of_int x2{2}))%W256))%PurePrimops
+                ((of_int 96))%W256 ((of_int y2{2}))%W256))%PurePrimops
+                  dest{1}
+            ((ConcretePrimops.ecAdd_precompile_unsafe_cast
+                ((of_int ((ZModField.asint x)))%W256,
+                  (of_int ((ZModField.asint y)))%W256)
+                ((of_int x2{2})%W256, (of_int y2{2})%W256))).`1))%PurePrimops
+        (dest{1} + (of_int 32)%W256)
+        ((ConcretePrimops.ecAdd_precompile_unsafe_cast
+            ((W256.of_int ((ZModField.asint x))),
+              (W256.of_int ((ZModField.asint y))))
+            ((of_int x2{2})%W256, (of_int y2{2})%W256))).`2)%PurePrimops
+    ). smt ().
+        rewrite /ecAdd_precompile_unsafe_cast in J0.
+        rewrite J0. progress.
+        rewrite to_uint_small. smt.
+        rewrite to_uint_small. smt.
+        rewrite to_uint_small. smt.
+        rewrite to_uint_small. smt.
+        rewrite F_eq_inzmod_asint F_eq_inzmod_asint H12.
+        rewrite odflt_some_eq proj1 proj2.
+        reflexivity.
+        seq 1 0 : (#pre). wp. skip. progress. rewrite PurePrimops.bit_andE. smt ().
+        rcondf {1} 1. progress. skip. progress. smt (). wp. skip. progress.
+        exists x. exists y. progress. exists x'. exists y'. progress.
+        seq 1 1 : (_16{1} = W256.zero /\ success{1} = W256.one /\ aresult{2} = None /\ !ConcretePrimops.staticcall_ec_add_should_succeed (W256.of_int (ZModField.asint x), W256.of_int (ZModField.asint y)) (W256.of_int x2v, W256.of_int y2v) /\ ConcretePrimops.staticcall_ec_mul_should_succeed (W256.of_int x1v, W256.of_int y1v) (W256.of_int sv)).
+        exists* Primops.memory{1}.
+        elim* => memory1.
+
+        call {1} (ConcretePrimops.staticcall_ec_add_pspec memory1 (W256.of_int (ZModField.asint x), W256.of_int (ZModField.asint y)) (W256.of_int x2v, W256.of_int y2v) W256.zero destu).
+        wp. skip. progress.
+
+        rewrite MemoryMap.load_store_diff. smt (@W256 @Utils). smt (@W256 @Utils).
+        rewrite MemoryMap.load_store_diff. smt (@W256 @Utils). smt (@W256 @Utils).
+        rewrite MemoryMap.load_store_diff. smt (@W256 @Utils). smt (@W256 @Utils).
+        smt (@MemoryMap).
+
+        rewrite MemoryMap.load_store_diff. smt (@W256 @Utils). smt (@W256 @Utils).
+        rewrite MemoryMap.load_store_diff. smt (@W256 @Utils). smt (@W256 @Utils).
+        smt (@MemoryMap).
+
+        rewrite MemoryMap.load_store_diff. smt (@W256 @Utils). smt (@W256 @Utils).
+        smt (@MemoryMap).
+
+        smt (@MemoryMap).
+
+        smt ().
+
+        apply eq_none_of_is_none.
+        have J0 := ConcretePrimops.ecAdd_precomp_is_none_of_should_not_succeed (W256.of_int (ZModField.asint x), W256.of_int (ZModField.asint y)) (W256.of_int x2{2}, W256.of_int y2{2}).
+        rewrite proj1 proj1 proj2 proj2 in J0.
+        rewrite to_uint_small in J0. smt.
+        rewrite to_uint_small in J0. smt.
+        rewrite to_uint_small in J0. smt.
+        rewrite to_uint_small in J0. smt.
+        rewrite F_eq_inzmod_asint F_eq_inzmod_asint in J0.
+        apply J0.
+        progress.
+        smt (@ZModField @EllipticCurve).
+        smt (@ZModField @EllipticCurve).
+
+        seq 1 1 :
+    (
+      _16{1} = W256.zero /\
+      success{1} = W256.zero /\
+      fresult{2} = None /\
+      ! (ConcretePrimops.staticcall_ec_add_should_succeed
+        ((of_int ((ZModField.asint x)))%W256,
+          (of_int ((ZModField.asint y)))%W256)
+        ((of_int x2v)%W256, (of_int y2v)%W256)) /\
+      (ConcretePrimops.staticcall_ec_mul_should_succeed ((of_int x1v)%W256, (of_int y1v)%W256)
+        ((of_int sv))%W256)
+    ).
+        wp. skip. progress. rewrite PurePrimops.bit_andE. smt ().
+        rcondt {1} 1. progress. skip. progress. smt (@W256).
+        inline *. wp. skip. progress. left. progress. exists x. exists y. smt ().
+        seq 1 1 : (success{1} = W256.zero /\ mresult{2} = None /\ !Primops.reverted{1} /\
+        ! (ConcretePrimops.staticcall_ec_mul_should_succeed ((of_int x1v)%W256, (of_int y1v)%W256)
+        ((of_int sv))%W256)).
+          exists* Primops.memory{1}.
+          elim*=>memory1. progress.
+
+          call {1} (ConcretePrimops.staticcall_ec_mul_pspec memory1 (W256.of_int x1v, W256.of_int y1v) (W256.of_int sv) W256.zero W256.zero). wp. skip. progress. 
+      
+    
+          rewrite MemoryMap.load_store_diff. smt (@W256 @Utils). smt (@W256 @Utils).
+          rewrite MemoryMap.load_store_diff. smt (@W256 @Utils). smt (@W256 @Utils).
+          smt (@MemoryMap).
+    
+          rewrite MemoryMap.load_store_diff. smt (@W256 @Utils). smt (@W256 @Utils).
+          smt (@MemoryMap).
+    
+          smt (@MemoryMap).
+    
+          smt ().
+
+          apply eq_none_of_is_none.
+
+          have J0 := ConcretePrimops.ecMul_precomp_is_none_of_should_not_succeed (W256.of_int x1{2}, W256.of_int y1{2}) (W256.of_int s{2}).
+          rewrite proj1 proj2 in J0.
+          rewrite to_uint_small in J0. smt.
+          rewrite to_uint_small in J0. smt.
+          rewrite to_uint_small in J0. smt.
+          apply J0. progress.
+          rcondf {2} 1. progress.
+          seq 7 1 :
+    (
+      success{1} = W256.zero /\
+      fresult{2} = None /\
+      !Primops.reverted{1} /\
+      ! (ConcretePrimops.staticcall_ec_mul_should_succeed ((of_int x1v)%W256, (of_int y1v)%W256)
+        ((of_int sv))%W256)
+    ). inline *. wp. skip. progress.
+        rewrite PurePrimops.bit_andE. smt ().
+        rewrite PurePrimops.bit_andE. smt ().
+        rewrite PurePrimops.bit_andE. smt ().
+        rewrite PurePrimops.bit_andE. smt ().
+        rewrite PurePrimops.bit_andE. smt ().
+        rewrite PurePrimops.bit_andE. smt ().
+        rcondt {1} 1. progress. skip. progress. smt (@W256 @PurePrimops).
+
+        inline *. wp. skip. progress. right. exact H0.
+    qed.
+    
+
+    
